cp with proof of rev

examples/seplogic/SL.Examples.fst
@@ -301,11 +301,14 @@ private let __elim_and (h:binder) :Tac unit
   = and_elim (pack (Tv_Var (bv_of_binder h)));
     clear h
 
-private let __elim_exists1 (h:binder) :Tac unit
+private let __elim_exists_return_binders1 (h:binder) :Tac (list binder)
   = let t = `__exists_elim_as_forall1 in
     apply_lemma (mk_e_app t [pack (Tv_Var (bv_of_binder h))]);
     clear h;
-    ignore (forall_intros ())
+    forall_intros ()
+
+private let __elim_exists1 (h:binder) :Tac unit
+  = ignore (__elim_exists_return_binders1 h)
 
 private let __elim_exists_return_binders2 (h:binder) :Tac (list binder)
   = let t = `__exists_elim_as_forall2 in
@@ -640,5 +643,156 @@ let rec append (l1 l2:listptr)
 		apply_lemma (`lemma_frame_out_empty_left);
 		smt ();
 		smt ();
-		smt ();
-                dump "A")
+		smt ())
+
+let lemma_apply_rewrite_assoc_mem1 (m1 m2 m3 m4:memory)
+  :Lemma (requires ((m2 <*> (m1 <*> m3)) == m4))
+         (ensures  ((m1 <*> (m2 <*> m3)) == m4))
+  = ()
+
+let rec rev_append (l1:listptr) (l2:listptr)
+  = (match l1 with
+     | None   -> l2
+     | Some r ->
+       let Cell hd tl = !r in
+       r := Cell hd l2;
+       rev_append tl l1)
+
+    <: STATE listptr (fun p m -> exists (fl1 fl2:list int) (m1 m2:memory).
+                                defined (m1 <*> m2) /\
+				m == (m1 <*> m2)    /\
+				valid l1 fl1 m1     /\
+				valid l2 fl2 m2     /\
+				(forall mf l. ((Set.equal (addrs_in mf) (Set.union (addrs_in m1) (addrs_in m2))) /\
+				          (valid l (List.Tot.rev_acc fl1 fl2) mf)) ==> p l mf))
+
+    by (fun () -> ignore (forall_intros ());
+               let h = implies_intro () in let l = __elim_exists_return_binders2 h in
+	       let fl1 = List.Tot.hd l in let fl2 = List.Tot.hd (List.Tot.tl l) in
+               let h = implies_intro () in let l = __elim_exists_return_binders2 h in
+	       let m1 = List.Tot.hd l in let m2 = List.Tot.hd (List.Tot.tl l) in
+	       let h = implies_intro () in __elim_and h; let h = implies_intro () in __elim_and h; let h = implies_intro () in __elim_and h; let h = implies_intro () in __elim_and h;
+	       ignore (implies_intro ());
+	       let h = implies_intro () in rewrite h;
+	       ignore (implies_intro ());
+
+               //induction on fl1
+	       apply_lemma (`__elim_valid_without_match);
+	       exact (quote l1); exact (binder_to_term fl1); exact (binder_to_term m1);
+	       split (); smt (); //send the valid on l1 goal to smt
+
+               split (); //split into base case and the inductive case
+
+               //base case, fl1 = []
+	       let h = implies_intro () in __elim_and h; let h = implies_intro () in __elim_and h;
+	       let h = implies_intro () in rewrite h; let h = implies_intro () in rewrite h; let h = implies_intro () in rewrite h;
+	       ignore (implies_intro ()); //valid assumption for l2
+	       ignore (implies_intro ()); //this is the forall mf f. keep an eye on it
+
+               split ();
+
+               ignore (implies_intro ());
+	       apply_lemma (`lemma_frame_out_empty_left);
+	       split (); smt ();
+	       ignore (implies_intro ()); ignore (forall_intro ()); ignore (implies_intro ()); ignore (forall_intro ()); ignore (implies_intro ());
+	       split (); smt ();
+	       apply_lemma (`lemma_frame_out_empty_left);
+	       smt ();
+
+               //inconsistent
+	       ignore (implies_intro ()); smt ();
+              
+               //inductive case fl1 is cons
+
+               let fl1_hd = forall_intro () in
+	       let fl1_tl = forall_intro () in
+	       let h = implies_intro () in __elim_and h; let h = implies_intro () in __elim_and h;
+	       let h = implies_intro () in rewrite h;
+	       ignore (implies_intro ());
+	       let h = implies_intro () in let l = __elim_exists_return_binders2 h in
+	       let l1_tl = List.Tot.hd l in let l1_tail_m = List.Tot.hd (List.Tot.tl l) in
+	       let h = implies_intro () in __elim_and h;
+	       let h = implies_intro () in rewrite h;
+	       ignore (implies_intro ()); ignore (implies_intro ());
+	       
+	       ignore (implies_intro ()); //this is forall mf l. assumption, keep an eye on it
+
+               split ();
+
+               //inconsistent
+	       ignore (implies_intro ());
+	       smt ();
+
+               ignore (implies_intro ());
+	       apply_lemma (`lemma_inline_in_patterns_two);
+	       split (); smt ();
+
+               split ();
+
+               ignore (implies_intro ());
+	       apply_lemma (`lemma_frame_out_empty_right);
+	       split (); smt ();
+
+               ignore (forall_intro ());
+	       let h = implies_intro () in rewrite h;
+	       norm [delta_only ["FStar.Pervasives.Native.__proj__Some__item__v"]];
+	       apply_lemma (`lemma_rewrite_sep_assoc4);
+	       apply_lemma (`lemma_rw); //!r in the Some branch
+	       split (); smt (); split (); smt ();
+	       apply_lemma (`lemma_frame_out_empty_right);
+	       split (); smt ();
+	       apply_lemma (`lemma_frame_out_empty_right);
+	       split (); smt ();
+	       ignore (forall_intros ()); ignore (implies_intro ());
+               apply_lemma (`lemma_rw); //r:= in the Some branch
+               split (); smt (); split (); smt ();
+
+               //give memory to the recursive call
+	       apply_lemma (`lemma_frame_out_empty_right);
+	       split (); smt ();
+
+               //partition the recursive call's memory and provide witnesses for existentials
+	       witness (binder_to_term fl1_tl);
+               //here i want: fl1_hd::fl2
+	       //mk_app `Cons (binder_to_term fl1_hd) (binder_to_term fl2)
+	       witness (mk_e_app (`Prims.Cons) [binder_to_term fl1_hd; binder_to_term fl2]);
+	       witness (binder_to_term l1_tail_m);
+	       let uv = uvar_env (cur_env ()) (Some (`SepLogic.Heap.memory)) in
+	       witness uv;
+	       split (); split (); split (); split ();
+	       flip ();
+               apply_lemma (`lemma_apply_rewrite_assoc_mem1);
+	       trefl ();
+	       smt ();
+	       smt ();
+	       smt ();
+
+	       ignore (forall_intros ()); ignore (implies_intros ());
+	       split (); smt (); split (); smt ();
+	       apply_lemma (`lemma_frame_out_empty_left);
+	       split (); smt (); split (); smt (); split (); smt (); split (); smt ();
+	       apply_lemma (`lemma_frame_out_empty_left);
+	       split (); smt (); split (); smt (); split (); smt ();
+	       apply_lemma (`lemma_frame_out_empty_left);
+	       smt (); smt ())
+
+let rev (l:listptr)
+  = (rev_append l None)
+
+    <: STATE listptr (fun p m -> exists fl. valid l fl m /\
+                                    (forall mf l. ((Set.equal (addrs_in m) (addrs_in mf)) /\
+				              (valid l (List.Tot.rev fl) mf)) ==> p l mf))
+
+    by (fun () -> ignore (forall_intro ());
+               let m = forall_intro () in
+	       let h = implies_intro () in let l = __elim_exists_return_binders1 h in
+	       let fl = List.Tot.hd l in
+	       let h = implies_intro () in __elim_and h;
+	       ignore (implies_intros ());
+
+               //provide existentials for the procedure call
+	       witness (binder_to_term fl);
+	       witness (`(Prims.Nil #int));
+	       witness (binder_to_term m);
+	       witness (`SepLogic.Heap.emp);
+	       smt ())
